% Auto-generated equations for algebra.
% This file is maintained by EquationGenerator.

\section*{Algebra}
\begin{align*}
\text{Example 1:}\quad (x + 1)^2 = x^2 + 2x + 1 \
\text{Example 2:}\quad (x + 2)^2 = x^2 + 4x + 4 \
\text{Example 3:}\quad (x + 3)^2 = x^2 + 6x + 9 \
\text{Example 4:}\quad (x + 4)^2 = x^2 + 8x + 16 \
\text{Example 5:}\quad (x + 5)^2 = x^2 + 10x + 25 \
\text{Example 6:}\quad (x + 6)^2 = x^2 + 12x + 36 \
\text{Example 7:}\quad (x + 7)^2 = x^2 + 14x + 49 \
\text{Example 8:}\quad (x + 8)^2 = x^2 + 16x + 64 \
\text{Example 9:}\quad (x + 9)^2 = x^2 + 18x + 81 \
\text{Example 10:}\quad (x + 10)^2 = x^2 + 20x + 100 \
\text{Example 11:}\quad (x + 11)^2 = x^2 + 22x + 121 \
\text{Example 12:}\quad (x + 12)^2 = x^2 + 24x + 144 \
\text{Example 13:}\quad (x + 13)^2 = x^2 + 26x + 169 \
\text{Example 14:}\quad (x + 14)^2 = x^2 + 28x + 196 \
\text{Example 15:}\quad (x + 15)^2 = x^2 + 30x + 225 \
\text{Example 16:}\quad (x + 16)^2 = x^2 + 32x + 256 \
\text{Example 17:}\quad (x + 17)^2 = x^2 + 34x + 289 \
\text{Example 18:}\quad (x + 18)^2 = x^2 + 36x + 324 \
\text{Example 19:}\quad (x + 19)^2 = x^2 + 38x + 361 \
\text{Example 20:}\quad (x + 20)^2 = x^2 + 40x + 400 \
\text{Example 21:}\quad (x + 21)^2 = x^2 + 42x + 441 \
\text{Example 22:}\quad (x + 22)^2 = x^2 + 44x + 484 \
\text{Example 23:}\quad (x + 23)^2 = x^2 + 46x + 529 \
\text{Example 24:}\quad (x + 24)^2 = x^2 + 48x + 576 \
\text{Example 25:}\quad (x + 25)^2 = x^2 + 50x + 625 \
\text{Example 26:}\quad (x + 26)^2 = x^2 + 52x + 676 \
\text{Example 27:}\quad (x + 27)^2 = x^2 + 54x + 729 \
\text{Example 28:}\quad (x + 28)^2 = x^2 + 56x + 784 \
\text{Example 29:}\quad (x + 29)^2 = x^2 + 58x + 841 \
\text{Example 30:}\quad (x + 30)^2 = x^2 + 60x + 900 \
\text{Example 31:}\quad (x + 31)^2 = x^2 + 62x + 961 \
\text{Example 32:}\quad (x + 32)^2 = x^2 + 64x + 1024 \
\text{Example 33:}\quad (x + 33)^2 = x^2 + 66x + 1089 \
\text{Example 34:}\quad (x + 34)^2 = x^2 + 68x + 1156 \
\text{Example 35:}\quad (x + 35)^2 = x^2 + 70x + 1225 \
\text{Example 36:}\quad (x + 36)^2 = x^2 + 72x + 1296 \
\text{Example 37:}\quad (x + 37)^2 = x^2 + 74x + 1369 \
\text{Example 38:}\quad (x + 38)^2 = x^2 + 76x + 1444 \
\text{Example 39:}\quad (x + 39)^2 = x^2 + 78x + 1521 \
\text{Example 40:}\quad (x + 40)^2 = x^2 + 80x + 1600 \
\text{Example 41:}\quad (x + 41)^2 = x^2 + 82x + 1681 \
\text{Example 42:}\quad (x + 42)^2 = x^2 + 84x + 1764 \
\text{Example 43:}\quad (x + 43)^2 = x^2 + 86x + 1849 \
\text{Example 44:}\quad (x + 44)^2 = x^2 + 88x + 1936 \
\text{Example 45:}\quad (x + 45)^2 = x^2 + 90x + 2025 \
\text{Example 46:}\quad (x + 46)^2 = x^2 + 92x + 2116 \
\text{Example 47:}\quad (x + 47)^2 = x^2 + 94x + 2209 \
\text{Example 48:}\quad (x + 48)^2 = x^2 + 96x + 2304 \
\text{Example 49:}\quad (x + 49)^2 = x^2 + 98x + 2401 \
\text{Example 50:}\quad (x + 50)^2 = x^2 + 100x + 2500 \
\text{Example 51:}\quad (x + 51)^2 = x^2 + 102x + 2601 \
\text{Example 52:}\quad (x + 52)^2 = x^2 + 104x + 2704 \
\text{Example 53:}\quad (x + 53)^2 = x^2 + 106x + 2809 \
\text{Example 54:}\quad (x + 54)^2 = x^2 + 108x + 2916 \
\text{Example 55:}\quad (x + 55)^2 = x^2 + 110x + 3025 \
\text{Example 56:}\quad (x + 56)^2 = x^2 + 112x + 3136 \
\text{Example 57:}\quad (x + 57)^2 = x^2 + 114x + 3249 \
\text{Example 58:}\quad (x + 58)^2 = x^2 + 116x + 3364 \
\text{Example 59:}\quad (x + 59)^2 = x^2 + 118x + 3481 \
\text{Example 60:}\quad (x + 60)^2 = x^2 + 120x + 3600 \
\text{Example 61:}\quad (x + 61)^2 = x^2 + 122x + 3721 \
\text{Example 62:}\quad (x + 62)^2 = x^2 + 124x + 3844 \
\text{Example 63:}\quad (x + 63)^2 = x^2 + 126x + 3969 \
\text{Example 64:}\quad (x + 64)^2 = x^2 + 128x + 4096 \
\text{Example 65:}\quad (x + 65)^2 = x^2 + 130x + 4225 \
\text{Example 66:}\quad (x + 66)^2 = x^2 + 132x + 4356 \
\text{Example 67:}\quad (x + 67)^2 = x^2 + 134x + 4489 \
\text{Example 68:}\quad (x + 68)^2 = x^2 + 136x + 4624 \
\text{Example 69:}\quad (x + 69)^2 = x^2 + 138x + 4761 \
\text{Example 70:}\quad (x + 70)^2 = x^2 + 140x + 4900 \
\text{Example 71:}\quad (x + 71)^2 = x^2 + 142x + 5041 \
\text{Example 72:}\quad (x + 72)^2 = x^2 + 144x + 5184 \
\text{Example 73:}\quad (x + 73)^2 = x^2 + 146x + 5329 \
\text{Example 74:}\quad (x + 74)^2 = x^2 + 148x + 5476 \
\text{Example 75:}\quad (x + 75)^2 = x^2 + 150x + 5625 \
\text{Example 76:}\quad (x + 76)^2 = x^2 + 152x + 5776 \
\text{Example 77:}\quad (x + 77)^2 = x^2 + 154x + 5929 \
\text{Example 78:}\quad (x + 78)^2 = x^2 + 156x + 6084 \
\text{Example 79:}\quad (x + 79)^2 = x^2 + 158x + 6241 \
\text{Example 80:}\quad (x + 80)^2 = x^2 + 160x + 6400 \
\text{Example 81:}\quad (x + 81)^2 = x^2 + 162x + 6561 \
\text{Example 82:}\quad (x + 82)^2 = x^2 + 164x + 6724 \
\text{Example 83:}\quad (x + 83)^2 = x^2 + 166x + 6889 \
\text{Example 84:}\quad (x + 84)^2 = x^2 + 168x + 7056 \
\text{Example 85:}\quad (x + 85)^2 = x^2 + 170x + 7225 \
\text{Example 86:}\quad (x + 86)^2 = x^2 + 172x + 7396 \
\text{Example 87:}\quad (x + 87)^2 = x^2 + 174x + 7569 \
\text{Example 88:}\quad (x + 88)^2 = x^2 + 176x + 7744 \
\text{Example 89:}\quad (x + 89)^2 = x^2 + 178x + 7921 \
\text{Example 90:}\quad (x + 90)^2 = x^2 + 180x + 8100 \
\text{Example 91:}\quad (x + 91)^2 = x^2 + 182x + 8281 \
\text{Example 92:}\quad (x + 92)^2 = x^2 + 184x + 8464 \
\text{Example 93:}\quad (x + 93)^2 = x^2 + 186x + 8649 \
\text{Example 94:}\quad (x + 94)^2 = x^2 + 188x + 8836 \
\text{Example 95:}\quad (x + 95)^2 = x^2 + 190x + 9025 \
\text{Example 96:}\quad (x + 96)^2 = x^2 + 192x + 9216 \
\text{Example 97:}\quad (x + 97)^2 = x^2 + 194x + 9409 \
\text{Example 98:}\quad (x + 98)^2 = x^2 + 196x + 9604 \
\text{Example 99:}\quad (x + 99)^2 = x^2 + 198x + 9801 \
\text{Example 100:}\quad (x + 100)^2 = x^2 + 200x + 10000 \
\text{Example 101:}\quad (x + 101)^2 = x^2 + 202x + 10201 \
\text{Example 102:}\quad (x + 102)^2 = x^2 + 204x + 10404 \
\text{Example 103:}\quad (x + 103)^2 = x^2 + 206x + 10609 \
\text{Example 104:}\quad (x + 104)^2 = x^2 + 208x + 10816 \
\text{Example 105:}\quad (x + 105)^2 = x^2 + 210x + 11025 \
\text{Example 106:}\quad (x + 106)^2 = x^2 + 212x + 11236 \
\text{Example 107:}\quad (x + 107)^2 = x^2 + 214x + 11449 \
\text{Example 108:}\quad (x + 108)^2 = x^2 + 216x + 11664 \
\text{Example 109:}\quad (x + 109)^2 = x^2 + 218x + 11881 \
\text{Example 110:}\quad (x + 110)^2 = x^2 + 220x + 12100 \
\text{Example 111:}\quad (x + 111)^2 = x^2 + 222x + 12321 \
\text{Example 112:}\quad (x + 112)^2 = x^2 + 224x + 12544 \
\text{Example 113:}\quad (x + 113)^2 = x^2 + 226x + 12769 \
\text{Example 114:}\quad (x + 114)^2 = x^2 + 228x + 12996 \
\text{Example 115:}\quad (x + 115)^2 = x^2 + 230x + 13225 \
\text{Example 116:}\quad (x + 116)^2 = x^2 + 232x + 13456 \
\text{Example 117:}\quad (x + 117)^2 = x^2 + 234x + 13689 \
\text{Example 118:}\quad (x + 118)^2 = x^2 + 236x + 13924 \
\text{Example 119:}\quad (x + 119)^2 = x^2 + 238x + 14161 \
\text{Example 120:}\quad (x + 120)^2 = x^2 + 240x + 14400 \
\text{Example 121:}\quad (x + 121)^2 = x^2 + 242x + 14641 \
\text{Example 122:}\quad (x + 122)^2 = x^2 + 244x + 14884 \
\text{Example 123:}\quad (x + 123)^2 = x^2 + 246x + 15129 \
\text{Example 124:}\quad (x + 124)^2 = x^2 + 248x + 15376 \
\text{Example 125:}\quad (x + 125)^2 = x^2 + 250x + 15625 \
\text{Example 126:}\quad (x + 126)^2 = x^2 + 252x + 15876 \
\text{Example 127:}\quad (x + 127)^2 = x^2 + 254x + 16129 \
\text{Example 128:}\quad (x + 128)^2 = x^2 + 256x + 16384 \
\text{Example 129:}\quad (x + 129)^2 = x^2 + 258x + 16641 \
\text{Example 130:}\quad (x + 130)^2 = x^2 + 260x + 16900 \
\text{Example 131:}\quad (x + 131)^2 = x^2 + 262x + 17161 \
\text{Example 132:}\quad (x + 132)^2 = x^2 + 264x + 17424 \
\text{Example 133:}\quad (x + 133)^2 = x^2 + 266x + 17689 \
\text{Example 134:}\quad (x + 134)^2 = x^2 + 268x + 17956 \
\text{Example 135:}\quad (x + 135)^2 = x^2 + 270x + 18225 \
\text{Example 136:}\quad (x + 136)^2 = x^2 + 272x + 18496 \
\text{Example 137:}\quad (x + 137)^2 = x^2 + 274x + 18769 \
\text{Example 138:}\quad (x + 138)^2 = x^2 + 276x + 19044 \
\text{Example 139:}\quad (x + 139)^2 = x^2 + 278x + 19321 \
\text{Example 140:}\quad (x + 140)^2 = x^2 + 280x + 19600 \
\text{Example 141:}\quad (x + 141)^2 = x^2 + 282x + 19881 \
\text{Example 142:}\quad (x + 142)^2 = x^2 + 284x + 20164 \
\text{Example 143:}\quad (x + 143)^2 = x^2 + 286x + 20449 \
\text{Example 144:}\quad (x + 144)^2 = x^2 + 288x + 20736 \
\text{Example 145:}\quad (x + 145)^2 = x^2 + 290x + 21025 \
\text{Example 146:}\quad (x + 146)^2 = x^2 + 292x + 21316 \
\text{Example 147:}\quad (x + 147)^2 = x^2 + 294x + 21609 \
\text{Example 148:}\quad (x + 148)^2 = x^2 + 296x + 21904 \
\text{Example 149:}\quad (x + 149)^2 = x^2 + 298x + 22201 \
\text{Example 150:}\quad (x + 150)^2 = x^2 + 300x + 22500 \
\text{Example 151:}\quad (x + 151)^2 = x^2 + 302x + 22801 \
\text{Example 152:}\quad (x + 152)^2 = x^2 + 304x + 23104 \
\text{Example 153:}\quad (x + 153)^2 = x^2 + 306x + 23409 \
\text{Example 154:}\quad (x + 154)^2 = x^2 + 308x + 23716 \
\text{Example 155:}\quad (x + 155)^2 = x^2 + 310x + 24025 \
\text{Example 156:}\quad (x + 156)^2 = x^2 + 312x + 24336 \
\text{Example 157:}\quad (x + 157)^2 = x^2 + 314x + 24649 \
\text{Example 158:}\quad (x + 158)^2 = x^2 + 316x + 24964 \
\text{Example 159:}\quad (x + 159)^2 = x^2 + 318x + 25281 \
\text{Example 160:}\quad (x + 160)^2 = x^2 + 320x + 25600 \
\text{Example 161:}\quad (x + 161)^2 = x^2 + 322x + 25921 \
\text{Example 162:}\quad (x + 162)^2 = x^2 + 324x + 26244 \
\text{Example 163:}\quad (x + 163)^2 = x^2 + 326x + 26569 \
\text{Example 164:}\quad (x + 164)^2 = x^2 + 328x + 26896 \
\text{Example 165:}\quad (x + 165)^2 = x^2 + 330x + 27225 \
\text{Example 166:}\quad (x + 166)^2 = x^2 + 332x + 27556 \
\text{Example 167:}\quad (x + 167)^2 = x^2 + 334x + 27889 \
\text{Example 168:}\quad (x + 168)^2 = x^2 + 336x + 28224 \
\text{Example 169:}\quad (x + 169)^2 = x^2 + 338x + 28561 \
\text{Example 170:}\quad (x + 170)^2 = x^2 + 340x + 28900 \
\text{Example 171:}\quad (x + 171)^2 = x^2 + 342x + 29241 \
\text{Example 172:}\quad (x + 172)^2 = x^2 + 344x + 29584 \
\text{Example 173:}\quad (x + 173)^2 = x^2 + 346x + 29929 \
\text{Example 174:}\quad (x + 174)^2 = x^2 + 348x + 30276 \
\text{Example 175:}\quad (x + 175)^2 = x^2 + 350x + 30625 \
\text{Example 176:}\quad (x + 176)^2 = x^2 + 352x + 30976 \
\text{Example 177:}\quad (x + 177)^2 = x^2 + 354x + 31329 \
\text{Example 178:}\quad (x + 178)^2 = x^2 + 356x + 31684 \
\text{Example 179:}\quad (x + 179)^2 = x^2 + 358x + 32041 \
\text{Example 180:}\quad (x + 180)^2 = x^2 + 360x + 32400 \
\end{align*}
