% Auto-generated equations for complex_numbers.
% This file is maintained by EquationGenerator.

\section*{Complex Numbers}
\begin{align*}
\text{Example 1:}\quad (a+bi)^1 = r^1(\cos(1\theta)+i\sin(1\theta)) \
\text{Example 2:}\quad (a+bi)^2 = r^2(\cos(2\theta)+i\sin(2\theta)) \
\text{Example 3:}\quad (a+bi)^3 = r^3(\cos(3\theta)+i\sin(3\theta)) \
\text{Example 4:}\quad (a+bi)^4 = r^4(\cos(4\theta)+i\sin(4\theta)) \
\text{Example 5:}\quad (a+bi)^5 = r^5(\cos(5\theta)+i\sin(5\theta)) \
\text{Example 6:}\quad (a+bi)^6 = r^6(\cos(6\theta)+i\sin(6\theta)) \
\text{Example 7:}\quad (a+bi)^7 = r^7(\cos(7\theta)+i\sin(7\theta)) \
\text{Example 8:}\quad (a+bi)^8 = r^8(\cos(8\theta)+i\sin(8\theta)) \
\text{Example 9:}\quad (a+bi)^9 = r^9(\cos(9\theta)+i\sin(9\theta)) \
\text{Example 10:}\quad (a+bi)^10 = r^10(\cos(10\theta)+i\sin(10\theta)) \
\text{Example 11:}\quad (a+bi)^11 = r^11(\cos(11\theta)+i\sin(11\theta)) \
\text{Example 12:}\quad (a+bi)^12 = r^12(\cos(12\theta)+i\sin(12\theta)) \
\text{Example 13:}\quad (a+bi)^13 = r^13(\cos(13\theta)+i\sin(13\theta)) \
\text{Example 14:}\quad (a+bi)^14 = r^14(\cos(14\theta)+i\sin(14\theta)) \
\text{Example 15:}\quad (a+bi)^15 = r^15(\cos(15\theta)+i\sin(15\theta)) \
\text{Example 16:}\quad (a+bi)^16 = r^16(\cos(16\theta)+i\sin(16\theta)) \
\text{Example 17:}\quad (a+bi)^17 = r^17(\cos(17\theta)+i\sin(17\theta)) \
\text{Example 18:}\quad (a+bi)^18 = r^18(\cos(18\theta)+i\sin(18\theta)) \
\text{Example 19:}\quad (a+bi)^19 = r^19(\cos(19\theta)+i\sin(19\theta)) \
\text{Example 20:}\quad (a+bi)^20 = r^20(\cos(20\theta)+i\sin(20\theta)) \
\text{Example 21:}\quad (a+bi)^21 = r^21(\cos(21\theta)+i\sin(21\theta)) \
\text{Example 22:}\quad (a+bi)^22 = r^22(\cos(22\theta)+i\sin(22\theta)) \
\text{Example 23:}\quad (a+bi)^23 = r^23(\cos(23\theta)+i\sin(23\theta)) \
\text{Example 24:}\quad (a+bi)^24 = r^24(\cos(24\theta)+i\sin(24\theta)) \
\text{Example 25:}\quad (a+bi)^25 = r^25(\cos(25\theta)+i\sin(25\theta)) \
\text{Example 26:}\quad (a+bi)^26 = r^26(\cos(26\theta)+i\sin(26\theta)) \
\text{Example 27:}\quad (a+bi)^27 = r^27(\cos(27\theta)+i\sin(27\theta)) \
\text{Example 28:}\quad (a+bi)^28 = r^28(\cos(28\theta)+i\sin(28\theta)) \
\text{Example 29:}\quad (a+bi)^29 = r^29(\cos(29\theta)+i\sin(29\theta)) \
\text{Example 30:}\quad (a+bi)^30 = r^30(\cos(30\theta)+i\sin(30\theta)) \
\text{Example 31:}\quad (a+bi)^31 = r^31(\cos(31\theta)+i\sin(31\theta)) \
\text{Example 32:}\quad (a+bi)^32 = r^32(\cos(32\theta)+i\sin(32\theta)) \
\text{Example 33:}\quad (a+bi)^33 = r^33(\cos(33\theta)+i\sin(33\theta)) \
\text{Example 34:}\quad (a+bi)^34 = r^34(\cos(34\theta)+i\sin(34\theta)) \
\text{Example 35:}\quad (a+bi)^35 = r^35(\cos(35\theta)+i\sin(35\theta)) \
\text{Example 36:}\quad (a+bi)^36 = r^36(\cos(36\theta)+i\sin(36\theta)) \
\text{Example 37:}\quad (a+bi)^37 = r^37(\cos(37\theta)+i\sin(37\theta)) \
\text{Example 38:}\quad (a+bi)^38 = r^38(\cos(38\theta)+i\sin(38\theta)) \
\text{Example 39:}\quad (a+bi)^39 = r^39(\cos(39\theta)+i\sin(39\theta)) \
\text{Example 40:}\quad (a+bi)^40 = r^40(\cos(40\theta)+i\sin(40\theta)) \
\text{Example 41:}\quad (a+bi)^41 = r^41(\cos(41\theta)+i\sin(41\theta)) \
\text{Example 42:}\quad (a+bi)^42 = r^42(\cos(42\theta)+i\sin(42\theta)) \
\text{Example 43:}\quad (a+bi)^43 = r^43(\cos(43\theta)+i\sin(43\theta)) \
\text{Example 44:}\quad (a+bi)^44 = r^44(\cos(44\theta)+i\sin(44\theta)) \
\text{Example 45:}\quad (a+bi)^45 = r^45(\cos(45\theta)+i\sin(45\theta)) \
\text{Example 46:}\quad (a+bi)^46 = r^46(\cos(46\theta)+i\sin(46\theta)) \
\text{Example 47:}\quad (a+bi)^47 = r^47(\cos(47\theta)+i\sin(47\theta)) \
\text{Example 48:}\quad (a+bi)^48 = r^48(\cos(48\theta)+i\sin(48\theta)) \
\text{Example 49:}\quad (a+bi)^49 = r^49(\cos(49\theta)+i\sin(49\theta)) \
\text{Example 50:}\quad (a+bi)^50 = r^50(\cos(50\theta)+i\sin(50\theta)) \
\text{Example 51:}\quad (a+bi)^51 = r^51(\cos(51\theta)+i\sin(51\theta)) \
\text{Example 52:}\quad (a+bi)^52 = r^52(\cos(52\theta)+i\sin(52\theta)) \
\text{Example 53:}\quad (a+bi)^53 = r^53(\cos(53\theta)+i\sin(53\theta)) \
\text{Example 54:}\quad (a+bi)^54 = r^54(\cos(54\theta)+i\sin(54\theta)) \
\text{Example 55:}\quad (a+bi)^55 = r^55(\cos(55\theta)+i\sin(55\theta)) \
\text{Example 56:}\quad (a+bi)^56 = r^56(\cos(56\theta)+i\sin(56\theta)) \
\text{Example 57:}\quad (a+bi)^57 = r^57(\cos(57\theta)+i\sin(57\theta)) \
\text{Example 58:}\quad (a+bi)^58 = r^58(\cos(58\theta)+i\sin(58\theta)) \
\text{Example 59:}\quad (a+bi)^59 = r^59(\cos(59\theta)+i\sin(59\theta)) \
\text{Example 60:}\quad (a+bi)^60 = r^60(\cos(60\theta)+i\sin(60\theta)) \
\text{Example 61:}\quad (a+bi)^61 = r^61(\cos(61\theta)+i\sin(61\theta)) \
\text{Example 62:}\quad (a+bi)^62 = r^62(\cos(62\theta)+i\sin(62\theta)) \
\text{Example 63:}\quad (a+bi)^63 = r^63(\cos(63\theta)+i\sin(63\theta)) \
\text{Example 64:}\quad (a+bi)^64 = r^64(\cos(64\theta)+i\sin(64\theta)) \
\text{Example 65:}\quad (a+bi)^65 = r^65(\cos(65\theta)+i\sin(65\theta)) \
\text{Example 66:}\quad (a+bi)^66 = r^66(\cos(66\theta)+i\sin(66\theta)) \
\text{Example 67:}\quad (a+bi)^67 = r^67(\cos(67\theta)+i\sin(67\theta)) \
\text{Example 68:}\quad (a+bi)^68 = r^68(\cos(68\theta)+i\sin(68\theta)) \
\text{Example 69:}\quad (a+bi)^69 = r^69(\cos(69\theta)+i\sin(69\theta)) \
\text{Example 70:}\quad (a+bi)^70 = r^70(\cos(70\theta)+i\sin(70\theta)) \
\text{Example 71:}\quad (a+bi)^71 = r^71(\cos(71\theta)+i\sin(71\theta)) \
\text{Example 72:}\quad (a+bi)^72 = r^72(\cos(72\theta)+i\sin(72\theta)) \
\text{Example 73:}\quad (a+bi)^73 = r^73(\cos(73\theta)+i\sin(73\theta)) \
\text{Example 74:}\quad (a+bi)^74 = r^74(\cos(74\theta)+i\sin(74\theta)) \
\text{Example 75:}\quad (a+bi)^75 = r^75(\cos(75\theta)+i\sin(75\theta)) \
\text{Example 76:}\quad (a+bi)^76 = r^76(\cos(76\theta)+i\sin(76\theta)) \
\text{Example 77:}\quad (a+bi)^77 = r^77(\cos(77\theta)+i\sin(77\theta)) \
\text{Example 78:}\quad (a+bi)^78 = r^78(\cos(78\theta)+i\sin(78\theta)) \
\text{Example 79:}\quad (a+bi)^79 = r^79(\cos(79\theta)+i\sin(79\theta)) \
\text{Example 80:}\quad (a+bi)^80 = r^80(\cos(80\theta)+i\sin(80\theta)) \
\text{Example 81:}\quad (a+bi)^81 = r^81(\cos(81\theta)+i\sin(81\theta)) \
\text{Example 82:}\quad (a+bi)^82 = r^82(\cos(82\theta)+i\sin(82\theta)) \
\text{Example 83:}\quad (a+bi)^83 = r^83(\cos(83\theta)+i\sin(83\theta)) \
\text{Example 84:}\quad (a+bi)^84 = r^84(\cos(84\theta)+i\sin(84\theta)) \
\text{Example 85:}\quad (a+bi)^85 = r^85(\cos(85\theta)+i\sin(85\theta)) \
\text{Example 86:}\quad (a+bi)^86 = r^86(\cos(86\theta)+i\sin(86\theta)) \
\text{Example 87:}\quad (a+bi)^87 = r^87(\cos(87\theta)+i\sin(87\theta)) \
\text{Example 88:}\quad (a+bi)^88 = r^88(\cos(88\theta)+i\sin(88\theta)) \
\text{Example 89:}\quad (a+bi)^89 = r^89(\cos(89\theta)+i\sin(89\theta)) \
\text{Example 90:}\quad (a+bi)^90 = r^90(\cos(90\theta)+i\sin(90\theta)) \
\text{Example 91:}\quad (a+bi)^91 = r^91(\cos(91\theta)+i\sin(91\theta)) \
\text{Example 92:}\quad (a+bi)^92 = r^92(\cos(92\theta)+i\sin(92\theta)) \
\text{Example 93:}\quad (a+bi)^93 = r^93(\cos(93\theta)+i\sin(93\theta)) \
\text{Example 94:}\quad (a+bi)^94 = r^94(\cos(94\theta)+i\sin(94\theta)) \
\text{Example 95:}\quad (a+bi)^95 = r^95(\cos(95\theta)+i\sin(95\theta)) \
\text{Example 96:}\quad (a+bi)^96 = r^96(\cos(96\theta)+i\sin(96\theta)) \
\text{Example 97:}\quad (a+bi)^97 = r^97(\cos(97\theta)+i\sin(97\theta)) \
\text{Example 98:}\quad (a+bi)^98 = r^98(\cos(98\theta)+i\sin(98\theta)) \
\text{Example 99:}\quad (a+bi)^99 = r^99(\cos(99\theta)+i\sin(99\theta)) \
\text{Example 100:}\quad (a+bi)^100 = r^100(\cos(100\theta)+i\sin(100\theta)) \
\text{Example 101:}\quad (a+bi)^101 = r^101(\cos(101\theta)+i\sin(101\theta)) \
\text{Example 102:}\quad (a+bi)^102 = r^102(\cos(102\theta)+i\sin(102\theta)) \
\text{Example 103:}\quad (a+bi)^103 = r^103(\cos(103\theta)+i\sin(103\theta)) \
\text{Example 104:}\quad (a+bi)^104 = r^104(\cos(104\theta)+i\sin(104\theta)) \
\text{Example 105:}\quad (a+bi)^105 = r^105(\cos(105\theta)+i\sin(105\theta)) \
\text{Example 106:}\quad (a+bi)^106 = r^106(\cos(106\theta)+i\sin(106\theta)) \
\text{Example 107:}\quad (a+bi)^107 = r^107(\cos(107\theta)+i\sin(107\theta)) \
\text{Example 108:}\quad (a+bi)^108 = r^108(\cos(108\theta)+i\sin(108\theta)) \
\text{Example 109:}\quad (a+bi)^109 = r^109(\cos(109\theta)+i\sin(109\theta)) \
\text{Example 110:}\quad (a+bi)^110 = r^110(\cos(110\theta)+i\sin(110\theta)) \
\text{Example 111:}\quad (a+bi)^111 = r^111(\cos(111\theta)+i\sin(111\theta)) \
\text{Example 112:}\quad (a+bi)^112 = r^112(\cos(112\theta)+i\sin(112\theta)) \
\text{Example 113:}\quad (a+bi)^113 = r^113(\cos(113\theta)+i\sin(113\theta)) \
\text{Example 114:}\quad (a+bi)^114 = r^114(\cos(114\theta)+i\sin(114\theta)) \
\text{Example 115:}\quad (a+bi)^115 = r^115(\cos(115\theta)+i\sin(115\theta)) \
\text{Example 116:}\quad (a+bi)^116 = r^116(\cos(116\theta)+i\sin(116\theta)) \
\text{Example 117:}\quad (a+bi)^117 = r^117(\cos(117\theta)+i\sin(117\theta)) \
\text{Example 118:}\quad (a+bi)^118 = r^118(\cos(118\theta)+i\sin(118\theta)) \
\text{Example 119:}\quad (a+bi)^119 = r^119(\cos(119\theta)+i\sin(119\theta)) \
\text{Example 120:}\quad (a+bi)^120 = r^120(\cos(120\theta)+i\sin(120\theta)) \
\text{Example 121:}\quad (a+bi)^121 = r^121(\cos(121\theta)+i\sin(121\theta)) \
\text{Example 122:}\quad (a+bi)^122 = r^122(\cos(122\theta)+i\sin(122\theta)) \
\text{Example 123:}\quad (a+bi)^123 = r^123(\cos(123\theta)+i\sin(123\theta)) \
\text{Example 124:}\quad (a+bi)^124 = r^124(\cos(124\theta)+i\sin(124\theta)) \
\text{Example 125:}\quad (a+bi)^125 = r^125(\cos(125\theta)+i\sin(125\theta)) \
\text{Example 126:}\quad (a+bi)^126 = r^126(\cos(126\theta)+i\sin(126\theta)) \
\text{Example 127:}\quad (a+bi)^127 = r^127(\cos(127\theta)+i\sin(127\theta)) \
\text{Example 128:}\quad (a+bi)^128 = r^128(\cos(128\theta)+i\sin(128\theta)) \
\text{Example 129:}\quad (a+bi)^129 = r^129(\cos(129\theta)+i\sin(129\theta)) \
\text{Example 130:}\quad (a+bi)^130 = r^130(\cos(130\theta)+i\sin(130\theta)) \
\text{Example 131:}\quad (a+bi)^131 = r^131(\cos(131\theta)+i\sin(131\theta)) \
\text{Example 132:}\quad (a+bi)^132 = r^132(\cos(132\theta)+i\sin(132\theta)) \
\text{Example 133:}\quad (a+bi)^133 = r^133(\cos(133\theta)+i\sin(133\theta)) \
\text{Example 134:}\quad (a+bi)^134 = r^134(\cos(134\theta)+i\sin(134\theta)) \
\text{Example 135:}\quad (a+bi)^135 = r^135(\cos(135\theta)+i\sin(135\theta)) \
\text{Example 136:}\quad (a+bi)^136 = r^136(\cos(136\theta)+i\sin(136\theta)) \
\text{Example 137:}\quad (a+bi)^137 = r^137(\cos(137\theta)+i\sin(137\theta)) \
\text{Example 138:}\quad (a+bi)^138 = r^138(\cos(138\theta)+i\sin(138\theta)) \
\text{Example 139:}\quad (a+bi)^139 = r^139(\cos(139\theta)+i\sin(139\theta)) \
\text{Example 140:}\quad (a+bi)^140 = r^140(\cos(140\theta)+i\sin(140\theta)) \
\text{Example 141:}\quad (a+bi)^141 = r^141(\cos(141\theta)+i\sin(141\theta)) \
\text{Example 142:}\quad (a+bi)^142 = r^142(\cos(142\theta)+i\sin(142\theta)) \
\text{Example 143:}\quad (a+bi)^143 = r^143(\cos(143\theta)+i\sin(143\theta)) \
\text{Example 144:}\quad (a+bi)^144 = r^144(\cos(144\theta)+i\sin(144\theta)) \
\text{Example 145:}\quad (a+bi)^145 = r^145(\cos(145\theta)+i\sin(145\theta)) \
\text{Example 146:}\quad (a+bi)^146 = r^146(\cos(146\theta)+i\sin(146\theta)) \
\text{Example 147:}\quad (a+bi)^147 = r^147(\cos(147\theta)+i\sin(147\theta)) \
\text{Example 148:}\quad (a+bi)^148 = r^148(\cos(148\theta)+i\sin(148\theta)) \
\text{Example 149:}\quad (a+bi)^149 = r^149(\cos(149\theta)+i\sin(149\theta)) \
\text{Example 150:}\quad (a+bi)^150 = r^150(\cos(150\theta)+i\sin(150\theta)) \
\text{Example 151:}\quad (a+bi)^151 = r^151(\cos(151\theta)+i\sin(151\theta)) \
\text{Example 152:}\quad (a+bi)^152 = r^152(\cos(152\theta)+i\sin(152\theta)) \
\text{Example 153:}\quad (a+bi)^153 = r^153(\cos(153\theta)+i\sin(153\theta)) \
\text{Example 154:}\quad (a+bi)^154 = r^154(\cos(154\theta)+i\sin(154\theta)) \
\text{Example 155:}\quad (a+bi)^155 = r^155(\cos(155\theta)+i\sin(155\theta)) \
\text{Example 156:}\quad (a+bi)^156 = r^156(\cos(156\theta)+i\sin(156\theta)) \
\text{Example 157:}\quad (a+bi)^157 = r^157(\cos(157\theta)+i\sin(157\theta)) \
\text{Example 158:}\quad (a+bi)^158 = r^158(\cos(158\theta)+i\sin(158\theta)) \
\text{Example 159:}\quad (a+bi)^159 = r^159(\cos(159\theta)+i\sin(159\theta)) \
\text{Example 160:}\quad (a+bi)^160 = r^160(\cos(160\theta)+i\sin(160\theta)) \
\text{Example 161:}\quad (a+bi)^161 = r^161(\cos(161\theta)+i\sin(161\theta)) \
\text{Example 162:}\quad (a+bi)^162 = r^162(\cos(162\theta)+i\sin(162\theta)) \
\text{Example 163:}\quad (a+bi)^163 = r^163(\cos(163\theta)+i\sin(163\theta)) \
\text{Example 164:}\quad (a+bi)^164 = r^164(\cos(164\theta)+i\sin(164\theta)) \
\text{Example 165:}\quad (a+bi)^165 = r^165(\cos(165\theta)+i\sin(165\theta)) \
\text{Example 166:}\quad (a+bi)^166 = r^166(\cos(166\theta)+i\sin(166\theta)) \
\text{Example 167:}\quad (a+bi)^167 = r^167(\cos(167\theta)+i\sin(167\theta)) \
\text{Example 168:}\quad (a+bi)^168 = r^168(\cos(168\theta)+i\sin(168\theta)) \
\text{Example 169:}\quad (a+bi)^169 = r^169(\cos(169\theta)+i\sin(169\theta)) \
\text{Example 170:}\quad (a+bi)^170 = r^170(\cos(170\theta)+i\sin(170\theta)) \
\text{Example 171:}\quad (a+bi)^171 = r^171(\cos(171\theta)+i\sin(171\theta)) \
\text{Example 172:}\quad (a+bi)^172 = r^172(\cos(172\theta)+i\sin(172\theta)) \
\text{Example 173:}\quad (a+bi)^173 = r^173(\cos(173\theta)+i\sin(173\theta)) \
\text{Example 174:}\quad (a+bi)^174 = r^174(\cos(174\theta)+i\sin(174\theta)) \
\text{Example 175:}\quad (a+bi)^175 = r^175(\cos(175\theta)+i\sin(175\theta)) \
\text{Example 176:}\quad (a+bi)^176 = r^176(\cos(176\theta)+i\sin(176\theta)) \
\text{Example 177:}\quad (a+bi)^177 = r^177(\cos(177\theta)+i\sin(177\theta)) \
\text{Example 178:}\quad (a+bi)^178 = r^178(\cos(178\theta)+i\sin(178\theta)) \
\text{Example 179:}\quad (a+bi)^179 = r^179(\cos(179\theta)+i\sin(179\theta)) \
\text{Example 180:}\quad (a+bi)^180 = r^180(\cos(180\theta)+i\sin(180\theta)) \
\end{align*}
