% Extended equation library appendix.
% Includes identities and sequences used for regression tests.

\section*{Equation Library Appendix}
\subsection*{Arithmetic Progressions}
\begin{align*}
S_{1} = 1 + 2 + \dots + 1 = \frac{1(1+1)}{2} \
S_{2} = 1 + 2 + \dots + 2 = \frac{2(2+1)}{2} \
S_{3} = 1 + 2 + \dots + 3 = \frac{3(3+1)}{2} \
S_{4} = 1 + 2 + \dots + 4 = \frac{4(4+1)}{2} \
S_{5} = 1 + 2 + \dots + 5 = \frac{5(5+1)}{2} \
S_{6} = 1 + 2 + \dots + 6 = \frac{6(6+1)}{2} \
S_{7} = 1 + 2 + \dots + 7 = \frac{7(7+1)}{2} \
S_{8} = 1 + 2 + \dots + 8 = \frac{8(8+1)}{2} \
S_{9} = 1 + 2 + \dots + 9 = \frac{9(9+1)}{2} \
S_{10} = 1 + 2 + \dots + 10 = \frac{10(10+1)}{2} \
S_{11} = 1 + 2 + \dots + 11 = \frac{11(11+1)}{2} \
S_{12} = 1 + 2 + \dots + 12 = \frac{12(12+1)}{2} \
S_{13} = 1 + 2 + \dots + 13 = \frac{13(13+1)}{2} \
S_{14} = 1 + 2 + \dots + 14 = \frac{14(14+1)}{2} \
S_{15} = 1 + 2 + \dots + 15 = \frac{15(15+1)}{2} \
S_{16} = 1 + 2 + \dots + 16 = \frac{16(16+1)}{2} \
S_{17} = 1 + 2 + \dots + 17 = \frac{17(17+1)}{2} \
S_{18} = 1 + 2 + \dots + 18 = \frac{18(18+1)}{2} \
S_{19} = 1 + 2 + \dots + 19 = \frac{19(19+1)}{2} \
S_{20} = 1 + 2 + \dots + 20 = \frac{20(20+1)}{2} \
S_{21} = 1 + 2 + \dots + 21 = \frac{21(21+1)}{2} \
S_{22} = 1 + 2 + \dots + 22 = \frac{22(22+1)}{2} \
S_{23} = 1 + 2 + \dots + 23 = \frac{23(23+1)}{2} \
S_{24} = 1 + 2 + \dots + 24 = \frac{24(24+1)}{2} \
S_{25} = 1 + 2 + \dots + 25 = \frac{25(25+1)}{2} \
S_{26} = 1 + 2 + \dots + 26 = \frac{26(26+1)}{2} \
S_{27} = 1 + 2 + \dots + 27 = \frac{27(27+1)}{2} \
S_{28} = 1 + 2 + \dots + 28 = \frac{28(28+1)}{2} \
S_{29} = 1 + 2 + \dots + 29 = \frac{29(29+1)}{2} \
S_{30} = 1 + 2 + \dots + 30 = \frac{30(30+1)}{2} \
S_{31} = 1 + 2 + \dots + 31 = \frac{31(31+1)}{2} \
S_{32} = 1 + 2 + \dots + 32 = \frac{32(32+1)}{2} \
S_{33} = 1 + 2 + \dots + 33 = \frac{33(33+1)}{2} \
S_{34} = 1 + 2 + \dots + 34 = \frac{34(34+1)}{2} \
S_{35} = 1 + 2 + \dots + 35 = \frac{35(35+1)}{2} \
S_{36} = 1 + 2 + \dots + 36 = \frac{36(36+1)}{2} \
S_{37} = 1 + 2 + \dots + 37 = \frac{37(37+1)}{2} \
S_{38} = 1 + 2 + \dots + 38 = \frac{38(38+1)}{2} \
S_{39} = 1 + 2 + \dots + 39 = \frac{39(39+1)}{2} \
S_{40} = 1 + 2 + \dots + 40 = \frac{40(40+1)}{2} \
S_{41} = 1 + 2 + \dots + 41 = \frac{41(41+1)}{2} \
S_{42} = 1 + 2 + \dots + 42 = \frac{42(42+1)}{2} \
S_{43} = 1 + 2 + \dots + 43 = \frac{43(43+1)}{2} \
S_{44} = 1 + 2 + \dots + 44 = \frac{44(44+1)}{2} \
S_{45} = 1 + 2 + \dots + 45 = \frac{45(45+1)}{2} \
S_{46} = 1 + 2 + \dots + 46 = \frac{46(46+1)}{2} \
S_{47} = 1 + 2 + \dots + 47 = \frac{47(47+1)}{2} \
S_{48} = 1 + 2 + \dots + 48 = \frac{48(48+1)}{2} \
S_{49} = 1 + 2 + \dots + 49 = \frac{49(49+1)}{2} \
S_{50} = 1 + 2 + \dots + 50 = \frac{50(50+1)}{2} \
S_{51} = 1 + 2 + \dots + 51 = \frac{51(51+1)}{2} \
S_{52} = 1 + 2 + \dots + 52 = \frac{52(52+1)}{2} \
S_{53} = 1 + 2 + \dots + 53 = \frac{53(53+1)}{2} \
S_{54} = 1 + 2 + \dots + 54 = \frac{54(54+1)}{2} \
S_{55} = 1 + 2 + \dots + 55 = \frac{55(55+1)}{2} \
S_{56} = 1 + 2 + \dots + 56 = \frac{56(56+1)}{2} \
S_{57} = 1 + 2 + \dots + 57 = \frac{57(57+1)}{2} \
S_{58} = 1 + 2 + \dots + 58 = \frac{58(58+1)}{2} \
S_{59} = 1 + 2 + \dots + 59 = \frac{59(59+1)}{2} \
S_{60} = 1 + 2 + \dots + 60 = \frac{60(60+1)}{2} \
S_{61} = 1 + 2 + \dots + 61 = \frac{61(61+1)}{2} \
S_{62} = 1 + 2 + \dots + 62 = \frac{62(62+1)}{2} \
S_{63} = 1 + 2 + \dots + 63 = \frac{63(63+1)}{2} \
S_{64} = 1 + 2 + \dots + 64 = \frac{64(64+1)}{2} \
S_{65} = 1 + 2 + \dots + 65 = \frac{65(65+1)}{2} \
S_{66} = 1 + 2 + \dots + 66 = \frac{66(66+1)}{2} \
S_{67} = 1 + 2 + \dots + 67 = \frac{67(67+1)}{2} \
S_{68} = 1 + 2 + \dots + 68 = \frac{68(68+1)}{2} \
S_{69} = 1 + 2 + \dots + 69 = \frac{69(69+1)}{2} \
S_{70} = 1 + 2 + \dots + 70 = \frac{70(70+1)}{2} \
S_{71} = 1 + 2 + \dots + 71 = \frac{71(71+1)}{2} \
S_{72} = 1 + 2 + \dots + 72 = \frac{72(72+1)}{2} \
S_{73} = 1 + 2 + \dots + 73 = \frac{73(73+1)}{2} \
S_{74} = 1 + 2 + \dots + 74 = \frac{74(74+1)}{2} \
S_{75} = 1 + 2 + \dots + 75 = \frac{75(75+1)}{2} \
S_{76} = 1 + 2 + \dots + 76 = \frac{76(76+1)}{2} \
S_{77} = 1 + 2 + \dots + 77 = \frac{77(77+1)}{2} \
S_{78} = 1 + 2 + \dots + 78 = \frac{78(78+1)}{2} \
S_{79} = 1 + 2 + \dots + 79 = \frac{79(79+1)}{2} \
S_{80} = 1 + 2 + \dots + 80 = \frac{80(80+1)}{2} \
S_{81} = 1 + 2 + \dots + 81 = \frac{81(81+1)}{2} \
S_{82} = 1 + 2 + \dots + 82 = \frac{82(82+1)}{2} \
S_{83} = 1 + 2 + \dots + 83 = \frac{83(83+1)}{2} \
S_{84} = 1 + 2 + \dots + 84 = \frac{84(84+1)}{2} \
S_{85} = 1 + 2 + \dots + 85 = \frac{85(85+1)}{2} \
S_{86} = 1 + 2 + \dots + 86 = \frac{86(86+1)}{2} \
S_{87} = 1 + 2 + \dots + 87 = \frac{87(87+1)}{2} \
S_{88} = 1 + 2 + \dots + 88 = \frac{88(88+1)}{2} \
S_{89} = 1 + 2 + \dots + 89 = \frac{89(89+1)}{2} \
S_{90} = 1 + 2 + \dots + 90 = \frac{90(90+1)}{2} \
S_{91} = 1 + 2 + \dots + 91 = \frac{91(91+1)}{2} \
S_{92} = 1 + 2 + \dots + 92 = \frac{92(92+1)}{2} \
S_{93} = 1 + 2 + \dots + 93 = \frac{93(93+1)}{2} \
S_{94} = 1 + 2 + \dots + 94 = \frac{94(94+1)}{2} \
S_{95} = 1 + 2 + \dots + 95 = \frac{95(95+1)}{2} \
S_{96} = 1 + 2 + \dots + 96 = \frac{96(96+1)}{2} \
S_{97} = 1 + 2 + \dots + 97 = \frac{97(97+1)}{2} \
S_{98} = 1 + 2 + \dots + 98 = \frac{98(98+1)}{2} \
S_{99} = 1 + 2 + \dots + 99 = \frac{99(99+1)}{2} \
S_{100} = 1 + 2 + \dots + 100 = \frac{100(100+1)}{2} \
S_{101} = 1 + 2 + \dots + 101 = \frac{101(101+1)}{2} \
S_{102} = 1 + 2 + \dots + 102 = \frac{102(102+1)}{2} \
S_{103} = 1 + 2 + \dots + 103 = \frac{103(103+1)}{2} \
S_{104} = 1 + 2 + \dots + 104 = \frac{104(104+1)}{2} \
S_{105} = 1 + 2 + \dots + 105 = \frac{105(105+1)}{2} \
S_{106} = 1 + 2 + \dots + 106 = \frac{106(106+1)}{2} \
S_{107} = 1 + 2 + \dots + 107 = \frac{107(107+1)}{2} \
S_{108} = 1 + 2 + \dots + 108 = \frac{108(108+1)}{2} \
S_{109} = 1 + 2 + \dots + 109 = \frac{109(109+1)}{2} \
S_{110} = 1 + 2 + \dots + 110 = \frac{110(110+1)}{2} \
S_{111} = 1 + 2 + \dots + 111 = \frac{111(111+1)}{2} \
S_{112} = 1 + 2 + \dots + 112 = \frac{112(112+1)}{2} \
S_{113} = 1 + 2 + \dots + 113 = \frac{113(113+1)}{2} \
S_{114} = 1 + 2 + \dots + 114 = \frac{114(114+1)}{2} \
S_{115} = 1 + 2 + \dots + 115 = \frac{115(115+1)}{2} \
S_{116} = 1 + 2 + \dots + 116 = \frac{116(116+1)}{2} \
S_{117} = 1 + 2 + \dots + 117 = \frac{117(117+1)}{2} \
S_{118} = 1 + 2 + \dots + 118 = \frac{118(118+1)}{2} \
S_{119} = 1 + 2 + \dots + 119 = \frac{119(119+1)}{2} \
S_{120} = 1 + 2 + \dots + 120 = \frac{120(120+1)}{2} \
\end{align*}

\subsection*{Geometric Progressions}
\begin{align*}
G_{1} = 1 + 2 + 2^2 + \dots + 2^{1} = 2^{1+1} - 1 \
G_{2} = 1 + 2 + 2^2 + \dots + 2^{2} = 2^{2+1} - 1 \
G_{3} = 1 + 2 + 2^2 + \dots + 2^{3} = 2^{3+1} - 1 \
G_{4} = 1 + 2 + 2^2 + \dots + 2^{4} = 2^{4+1} - 1 \
G_{5} = 1 + 2 + 2^2 + \dots + 2^{5} = 2^{5+1} - 1 \
G_{6} = 1 + 2 + 2^2 + \dots + 2^{6} = 2^{6+1} - 1 \
G_{7} = 1 + 2 + 2^2 + \dots + 2^{7} = 2^{7+1} - 1 \
G_{8} = 1 + 2 + 2^2 + \dots + 2^{8} = 2^{8+1} - 1 \
G_{9} = 1 + 2 + 2^2 + \dots + 2^{9} = 2^{9+1} - 1 \
G_{10} = 1 + 2 + 2^2 + \dots + 2^{10} = 2^{10+1} - 1 \
G_{11} = 1 + 2 + 2^2 + \dots + 2^{11} = 2^{11+1} - 1 \
G_{12} = 1 + 2 + 2^2 + \dots + 2^{12} = 2^{12+1} - 1 \
G_{13} = 1 + 2 + 2^2 + \dots + 2^{13} = 2^{13+1} - 1 \
G_{14} = 1 + 2 + 2^2 + \dots + 2^{14} = 2^{14+1} - 1 \
G_{15} = 1 + 2 + 2^2 + \dots + 2^{15} = 2^{15+1} - 1 \
G_{16} = 1 + 2 + 2^2 + \dots + 2^{16} = 2^{16+1} - 1 \
G_{17} = 1 + 2 + 2^2 + \dots + 2^{17} = 2^{17+1} - 1 \
G_{18} = 1 + 2 + 2^2 + \dots + 2^{18} = 2^{18+1} - 1 \
G_{19} = 1 + 2 + 2^2 + \dots + 2^{19} = 2^{19+1} - 1 \
G_{20} = 1 + 2 + 2^2 + \dots + 2^{20} = 2^{20+1} - 1 \
G_{21} = 1 + 2 + 2^2 + \dots + 2^{21} = 2^{21+1} - 1 \
G_{22} = 1 + 2 + 2^2 + \dots + 2^{22} = 2^{22+1} - 1 \
G_{23} = 1 + 2 + 2^2 + \dots + 2^{23} = 2^{23+1} - 1 \
G_{24} = 1 + 2 + 2^2 + \dots + 2^{24} = 2^{24+1} - 1 \
G_{25} = 1 + 2 + 2^2 + \dots + 2^{25} = 2^{25+1} - 1 \
G_{26} = 1 + 2 + 2^2 + \dots + 2^{26} = 2^{26+1} - 1 \
G_{27} = 1 + 2 + 2^2 + \dots + 2^{27} = 2^{27+1} - 1 \
G_{28} = 1 + 2 + 2^2 + \dots + 2^{28} = 2^{28+1} - 1 \
G_{29} = 1 + 2 + 2^2 + \dots + 2^{29} = 2^{29+1} - 1 \
G_{30} = 1 + 2 + 2^2 + \dots + 2^{30} = 2^{30+1} - 1 \
G_{31} = 1 + 2 + 2^2 + \dots + 2^{31} = 2^{31+1} - 1 \
G_{32} = 1 + 2 + 2^2 + \dots + 2^{32} = 2^{32+1} - 1 \
G_{33} = 1 + 2 + 2^2 + \dots + 2^{33} = 2^{33+1} - 1 \
G_{34} = 1 + 2 + 2^2 + \dots + 2^{34} = 2^{34+1} - 1 \
G_{35} = 1 + 2 + 2^2 + \dots + 2^{35} = 2^{35+1} - 1 \
G_{36} = 1 + 2 + 2^2 + \dots + 2^{36} = 2^{36+1} - 1 \
G_{37} = 1 + 2 + 2^2 + \dots + 2^{37} = 2^{37+1} - 1 \
G_{38} = 1 + 2 + 2^2 + \dots + 2^{38} = 2^{38+1} - 1 \
G_{39} = 1 + 2 + 2^2 + \dots + 2^{39} = 2^{39+1} - 1 \
G_{40} = 1 + 2 + 2^2 + \dots + 2^{40} = 2^{40+1} - 1 \
G_{41} = 1 + 2 + 2^2 + \dots + 2^{41} = 2^{41+1} - 1 \
G_{42} = 1 + 2 + 2^2 + \dots + 2^{42} = 2^{42+1} - 1 \
G_{43} = 1 + 2 + 2^2 + \dots + 2^{43} = 2^{43+1} - 1 \
G_{44} = 1 + 2 + 2^2 + \dots + 2^{44} = 2^{44+1} - 1 \
G_{45} = 1 + 2 + 2^2 + \dots + 2^{45} = 2^{45+1} - 1 \
G_{46} = 1 + 2 + 2^2 + \dots + 2^{46} = 2^{46+1} - 1 \
G_{47} = 1 + 2 + 2^2 + \dots + 2^{47} = 2^{47+1} - 1 \
G_{48} = 1 + 2 + 2^2 + \dots + 2^{48} = 2^{48+1} - 1 \
G_{49} = 1 + 2 + 2^2 + \dots + 2^{49} = 2^{49+1} - 1 \
G_{50} = 1 + 2 + 2^2 + \dots + 2^{50} = 2^{50+1} - 1 \
G_{51} = 1 + 2 + 2^2 + \dots + 2^{51} = 2^{51+1} - 1 \
G_{52} = 1 + 2 + 2^2 + \dots + 2^{52} = 2^{52+1} - 1 \
G_{53} = 1 + 2 + 2^2 + \dots + 2^{53} = 2^{53+1} - 1 \
G_{54} = 1 + 2 + 2^2 + \dots + 2^{54} = 2^{54+1} - 1 \
G_{55} = 1 + 2 + 2^2 + \dots + 2^{55} = 2^{55+1} - 1 \
G_{56} = 1 + 2 + 2^2 + \dots + 2^{56} = 2^{56+1} - 1 \
G_{57} = 1 + 2 + 2^2 + \dots + 2^{57} = 2^{57+1} - 1 \
G_{58} = 1 + 2 + 2^2 + \dots + 2^{58} = 2^{58+1} - 1 \
G_{59} = 1 + 2 + 2^2 + \dots + 2^{59} = 2^{59+1} - 1 \
G_{60} = 1 + 2 + 2^2 + \dots + 2^{60} = 2^{60+1} - 1 \
G_{61} = 1 + 2 + 2^2 + \dots + 2^{61} = 2^{61+1} - 1 \
G_{62} = 1 + 2 + 2^2 + \dots + 2^{62} = 2^{62+1} - 1 \
G_{63} = 1 + 2 + 2^2 + \dots + 2^{63} = 2^{63+1} - 1 \
G_{64} = 1 + 2 + 2^2 + \dots + 2^{64} = 2^{64+1} - 1 \
G_{65} = 1 + 2 + 2^2 + \dots + 2^{65} = 2^{65+1} - 1 \
G_{66} = 1 + 2 + 2^2 + \dots + 2^{66} = 2^{66+1} - 1 \
G_{67} = 1 + 2 + 2^2 + \dots + 2^{67} = 2^{67+1} - 1 \
G_{68} = 1 + 2 + 2^2 + \dots + 2^{68} = 2^{68+1} - 1 \
G_{69} = 1 + 2 + 2^2 + \dots + 2^{69} = 2^{69+1} - 1 \
G_{70} = 1 + 2 + 2^2 + \dots + 2^{70} = 2^{70+1} - 1 \
G_{71} = 1 + 2 + 2^2 + \dots + 2^{71} = 2^{71+1} - 1 \
G_{72} = 1 + 2 + 2^2 + \dots + 2^{72} = 2^{72+1} - 1 \
G_{73} = 1 + 2 + 2^2 + \dots + 2^{73} = 2^{73+1} - 1 \
G_{74} = 1 + 2 + 2^2 + \dots + 2^{74} = 2^{74+1} - 1 \
G_{75} = 1 + 2 + 2^2 + \dots + 2^{75} = 2^{75+1} - 1 \
G_{76} = 1 + 2 + 2^2 + \dots + 2^{76} = 2^{76+1} - 1 \
G_{77} = 1 + 2 + 2^2 + \dots + 2^{77} = 2^{77+1} - 1 \
G_{78} = 1 + 2 + 2^2 + \dots + 2^{78} = 2^{78+1} - 1 \
G_{79} = 1 + 2 + 2^2 + \dots + 2^{79} = 2^{79+1} - 1 \
G_{80} = 1 + 2 + 2^2 + \dots + 2^{80} = 2^{80+1} - 1 \
G_{81} = 1 + 2 + 2^2 + \dots + 2^{81} = 2^{81+1} - 1 \
G_{82} = 1 + 2 + 2^2 + \dots + 2^{82} = 2^{82+1} - 1 \
G_{83} = 1 + 2 + 2^2 + \dots + 2^{83} = 2^{83+1} - 1 \
G_{84} = 1 + 2 + 2^2 + \dots + 2^{84} = 2^{84+1} - 1 \
G_{85} = 1 + 2 + 2^2 + \dots + 2^{85} = 2^{85+1} - 1 \
G_{86} = 1 + 2 + 2^2 + \dots + 2^{86} = 2^{86+1} - 1 \
G_{87} = 1 + 2 + 2^2 + \dots + 2^{87} = 2^{87+1} - 1 \
G_{88} = 1 + 2 + 2^2 + \dots + 2^{88} = 2^{88+1} - 1 \
G_{89} = 1 + 2 + 2^2 + \dots + 2^{89} = 2^{89+1} - 1 \
G_{90} = 1 + 2 + 2^2 + \dots + 2^{90} = 2^{90+1} - 1 \
G_{91} = 1 + 2 + 2^2 + \dots + 2^{91} = 2^{91+1} - 1 \
G_{92} = 1 + 2 + 2^2 + \dots + 2^{92} = 2^{92+1} - 1 \
G_{93} = 1 + 2 + 2^2 + \dots + 2^{93} = 2^{93+1} - 1 \
G_{94} = 1 + 2 + 2^2 + \dots + 2^{94} = 2^{94+1} - 1 \
G_{95} = 1 + 2 + 2^2 + \dots + 2^{95} = 2^{95+1} - 1 \
G_{96} = 1 + 2 + 2^2 + \dots + 2^{96} = 2^{96+1} - 1 \
G_{97} = 1 + 2 + 2^2 + \dots + 2^{97} = 2^{97+1} - 1 \
G_{98} = 1 + 2 + 2^2 + \dots + 2^{98} = 2^{98+1} - 1 \
G_{99} = 1 + 2 + 2^2 + \dots + 2^{99} = 2^{99+1} - 1 \
G_{100} = 1 + 2 + 2^2 + \dots + 2^{100} = 2^{100+1} - 1 \
G_{101} = 1 + 2 + 2^2 + \dots + 2^{101} = 2^{101+1} - 1 \
G_{102} = 1 + 2 + 2^2 + \dots + 2^{102} = 2^{102+1} - 1 \
G_{103} = 1 + 2 + 2^2 + \dots + 2^{103} = 2^{103+1} - 1 \
G_{104} = 1 + 2 + 2^2 + \dots + 2^{104} = 2^{104+1} - 1 \
G_{105} = 1 + 2 + 2^2 + \dots + 2^{105} = 2^{105+1} - 1 \
G_{106} = 1 + 2 + 2^2 + \dots + 2^{106} = 2^{106+1} - 1 \
G_{107} = 1 + 2 + 2^2 + \dots + 2^{107} = 2^{107+1} - 1 \
G_{108} = 1 + 2 + 2^2 + \dots + 2^{108} = 2^{108+1} - 1 \
G_{109} = 1 + 2 + 2^2 + \dots + 2^{109} = 2^{109+1} - 1 \
G_{110} = 1 + 2 + 2^2 + \dots + 2^{110} = 2^{110+1} - 1 \
G_{111} = 1 + 2 + 2^2 + \dots + 2^{111} = 2^{111+1} - 1 \
G_{112} = 1 + 2 + 2^2 + \dots + 2^{112} = 2^{112+1} - 1 \
G_{113} = 1 + 2 + 2^2 + \dots + 2^{113} = 2^{113+1} - 1 \
G_{114} = 1 + 2 + 2^2 + \dots + 2^{114} = 2^{114+1} - 1 \
G_{115} = 1 + 2 + 2^2 + \dots + 2^{115} = 2^{115+1} - 1 \
G_{116} = 1 + 2 + 2^2 + \dots + 2^{116} = 2^{116+1} - 1 \
G_{117} = 1 + 2 + 2^2 + \dots + 2^{117} = 2^{117+1} - 1 \
G_{118} = 1 + 2 + 2^2 + \dots + 2^{118} = 2^{118+1} - 1 \
G_{119} = 1 + 2 + 2^2 + \dots + 2^{119} = 2^{119+1} - 1 \
G_{120} = 1 + 2 + 2^2 + \dots + 2^{120} = 2^{120+1} - 1 \
\end{align*}

\subsection*{Binomial Expansions}
\begin{align*}
(x + 1)^{1} = \sum_{k=0}^{1} \binom{1}{k} x^k \
(x + 1)^{2} = \sum_{k=0}^{2} \binom{2}{k} x^k \
(x + 1)^{3} = \sum_{k=0}^{3} \binom{3}{k} x^k \
(x + 1)^{4} = \sum_{k=0}^{4} \binom{4}{k} x^k \
(x + 1)^{5} = \sum_{k=0}^{5} \binom{5}{k} x^k \
(x + 1)^{6} = \sum_{k=0}^{6} \binom{6}{k} x^k \
(x + 1)^{7} = \sum_{k=0}^{7} \binom{7}{k} x^k \
(x + 1)^{8} = \sum_{k=0}^{8} \binom{8}{k} x^k \
(x + 1)^{9} = \sum_{k=0}^{9} \binom{9}{k} x^k \
(x + 1)^{10} = \sum_{k=0}^{10} \binom{10}{k} x^k \
(x + 1)^{11} = \sum_{k=0}^{11} \binom{11}{k} x^k \
(x + 1)^{12} = \sum_{k=0}^{12} \binom{12}{k} x^k \
(x + 1)^{13} = \sum_{k=0}^{13} \binom{13}{k} x^k \
(x + 1)^{14} = \sum_{k=0}^{14} \binom{14}{k} x^k \
(x + 1)^{15} = \sum_{k=0}^{15} \binom{15}{k} x^k \
(x + 1)^{16} = \sum_{k=0}^{16} \binom{16}{k} x^k \
(x + 1)^{17} = \sum_{k=0}^{17} \binom{17}{k} x^k \
(x + 1)^{18} = \sum_{k=0}^{18} \binom{18}{k} x^k \
(x + 1)^{19} = \sum_{k=0}^{19} \binom{19}{k} x^k \
(x + 1)^{20} = \sum_{k=0}^{20} \binom{20}{k} x^k \
(x + 1)^{21} = \sum_{k=0}^{21} \binom{21}{k} x^k \
(x + 1)^{22} = \sum_{k=0}^{22} \binom{22}{k} x^k \
(x + 1)^{23} = \sum_{k=0}^{23} \binom{23}{k} x^k \
(x + 1)^{24} = \sum_{k=0}^{24} \binom{24}{k} x^k \
(x + 1)^{25} = \sum_{k=0}^{25} \binom{25}{k} x^k \
(x + 1)^{26} = \sum_{k=0}^{26} \binom{26}{k} x^k \
(x + 1)^{27} = \sum_{k=0}^{27} \binom{27}{k} x^k \
(x + 1)^{28} = \sum_{k=0}^{28} \binom{28}{k} x^k \
(x + 1)^{29} = \sum_{k=0}^{29} \binom{29}{k} x^k \
(x + 1)^{30} = \sum_{k=0}^{30} \binom{30}{k} x^k \
(x + 1)^{31} = \sum_{k=0}^{31} \binom{31}{k} x^k \
(x + 1)^{32} = \sum_{k=0}^{32} \binom{32}{k} x^k \
(x + 1)^{33} = \sum_{k=0}^{33} \binom{33}{k} x^k \
(x + 1)^{34} = \sum_{k=0}^{34} \binom{34}{k} x^k \
(x + 1)^{35} = \sum_{k=0}^{35} \binom{35}{k} x^k \
(x + 1)^{36} = \sum_{k=0}^{36} \binom{36}{k} x^k \
(x + 1)^{37} = \sum_{k=0}^{37} \binom{37}{k} x^k \
(x + 1)^{38} = \sum_{k=0}^{38} \binom{38}{k} x^k \
(x + 1)^{39} = \sum_{k=0}^{39} \binom{39}{k} x^k \
(x + 1)^{40} = \sum_{k=0}^{40} \binom{40}{k} x^k \
(x + 1)^{41} = \sum_{k=0}^{41} \binom{41}{k} x^k \
(x + 1)^{42} = \sum_{k=0}^{42} \binom{42}{k} x^k \
(x + 1)^{43} = \sum_{k=0}^{43} \binom{43}{k} x^k \
(x + 1)^{44} = \sum_{k=0}^{44} \binom{44}{k} x^k \
(x + 1)^{45} = \sum_{k=0}^{45} \binom{45}{k} x^k \
(x + 1)^{46} = \sum_{k=0}^{46} \binom{46}{k} x^k \
(x + 1)^{47} = \sum_{k=0}^{47} \binom{47}{k} x^k \
(x + 1)^{48} = \sum_{k=0}^{48} \binom{48}{k} x^k \
(x + 1)^{49} = \sum_{k=0}^{49} \binom{49}{k} x^k \
(x + 1)^{50} = \sum_{k=0}^{50} \binom{50}{k} x^k \
(x + 1)^{51} = \sum_{k=0}^{51} \binom{51}{k} x^k \
(x + 1)^{52} = \sum_{k=0}^{52} \binom{52}{k} x^k \
(x + 1)^{53} = \sum_{k=0}^{53} \binom{53}{k} x^k \
(x + 1)^{54} = \sum_{k=0}^{54} \binom{54}{k} x^k \
(x + 1)^{55} = \sum_{k=0}^{55} \binom{55}{k} x^k \
(x + 1)^{56} = \sum_{k=0}^{56} \binom{56}{k} x^k \
(x + 1)^{57} = \sum_{k=0}^{57} \binom{57}{k} x^k \
(x + 1)^{58} = \sum_{k=0}^{58} \binom{58}{k} x^k \
(x + 1)^{59} = \sum_{k=0}^{59} \binom{59}{k} x^k \
(x + 1)^{60} = \sum_{k=0}^{60} \binom{60}{k} x^k \
(x + 1)^{61} = \sum_{k=0}^{61} \binom{61}{k} x^k \
(x + 1)^{62} = \sum_{k=0}^{62} \binom{62}{k} x^k \
(x + 1)^{63} = \sum_{k=0}^{63} \binom{63}{k} x^k \
(x + 1)^{64} = \sum_{k=0}^{64} \binom{64}{k} x^k \
(x + 1)^{65} = \sum_{k=0}^{65} \binom{65}{k} x^k \
(x + 1)^{66} = \sum_{k=0}^{66} \binom{66}{k} x^k \
(x + 1)^{67} = \sum_{k=0}^{67} \binom{67}{k} x^k \
(x + 1)^{68} = \sum_{k=0}^{68} \binom{68}{k} x^k \
(x + 1)^{69} = \sum_{k=0}^{69} \binom{69}{k} x^k \
(x + 1)^{70} = \sum_{k=0}^{70} \binom{70}{k} x^k \
(x + 1)^{71} = \sum_{k=0}^{71} \binom{71}{k} x^k \
(x + 1)^{72} = \sum_{k=0}^{72} \binom{72}{k} x^k \
(x + 1)^{73} = \sum_{k=0}^{73} \binom{73}{k} x^k \
(x + 1)^{74} = \sum_{k=0}^{74} \binom{74}{k} x^k \
(x + 1)^{75} = \sum_{k=0}^{75} \binom{75}{k} x^k \
(x + 1)^{76} = \sum_{k=0}^{76} \binom{76}{k} x^k \
(x + 1)^{77} = \sum_{k=0}^{77} \binom{77}{k} x^k \
(x + 1)^{78} = \sum_{k=0}^{78} \binom{78}{k} x^k \
(x + 1)^{79} = \sum_{k=0}^{79} \binom{79}{k} x^k \
(x + 1)^{80} = \sum_{k=0}^{80} \binom{80}{k} x^k \
(x + 1)^{81} = \sum_{k=0}^{81} \binom{81}{k} x^k \
(x + 1)^{82} = \sum_{k=0}^{82} \binom{82}{k} x^k \
(x + 1)^{83} = \sum_{k=0}^{83} \binom{83}{k} x^k \
(x + 1)^{84} = \sum_{k=0}^{84} \binom{84}{k} x^k \
(x + 1)^{85} = \sum_{k=0}^{85} \binom{85}{k} x^k \
(x + 1)^{86} = \sum_{k=0}^{86} \binom{86}{k} x^k \
(x + 1)^{87} = \sum_{k=0}^{87} \binom{87}{k} x^k \
(x + 1)^{88} = \sum_{k=0}^{88} \binom{88}{k} x^k \
(x + 1)^{89} = \sum_{k=0}^{89} \binom{89}{k} x^k \
(x + 1)^{90} = \sum_{k=0}^{90} \binom{90}{k} x^k \
(x + 1)^{91} = \sum_{k=0}^{91} \binom{91}{k} x^k \
(x + 1)^{92} = \sum_{k=0}^{92} \binom{92}{k} x^k \
(x + 1)^{93} = \sum_{k=0}^{93} \binom{93}{k} x^k \
(x + 1)^{94} = \sum_{k=0}^{94} \binom{94}{k} x^k \
(x + 1)^{95} = \sum_{k=0}^{95} \binom{95}{k} x^k \
(x + 1)^{96} = \sum_{k=0}^{96} \binom{96}{k} x^k \
(x + 1)^{97} = \sum_{k=0}^{97} \binom{97}{k} x^k \
(x + 1)^{98} = \sum_{k=0}^{98} \binom{98}{k} x^k \
(x + 1)^{99} = \sum_{k=0}^{99} \binom{99}{k} x^k \
(x + 1)^{100} = \sum_{k=0}^{100} \binom{100}{k} x^k \
(x + 1)^{101} = \sum_{k=0}^{101} \binom{101}{k} x^k \
(x + 1)^{102} = \sum_{k=0}^{102} \binom{102}{k} x^k \
(x + 1)^{103} = \sum_{k=0}^{103} \binom{103}{k} x^k \
(x + 1)^{104} = \sum_{k=0}^{104} \binom{104}{k} x^k \
(x + 1)^{105} = \sum_{k=0}^{105} \binom{105}{k} x^k \
(x + 1)^{106} = \sum_{k=0}^{106} \binom{106}{k} x^k \
(x + 1)^{107} = \sum_{k=0}^{107} \binom{107}{k} x^k \
(x + 1)^{108} = \sum_{k=0}^{108} \binom{108}{k} x^k \
(x + 1)^{109} = \sum_{k=0}^{109} \binom{109}{k} x^k \
(x + 1)^{110} = \sum_{k=0}^{110} \binom{110}{k} x^k \
(x + 1)^{111} = \sum_{k=0}^{111} \binom{111}{k} x^k \
(x + 1)^{112} = \sum_{k=0}^{112} \binom{112}{k} x^k \
(x + 1)^{113} = \sum_{k=0}^{113} \binom{113}{k} x^k \
(x + 1)^{114} = \sum_{k=0}^{114} \binom{114}{k} x^k \
(x + 1)^{115} = \sum_{k=0}^{115} \binom{115}{k} x^k \
(x + 1)^{116} = \sum_{k=0}^{116} \binom{116}{k} x^k \
(x + 1)^{117} = \sum_{k=0}^{117} \binom{117}{k} x^k \
(x + 1)^{118} = \sum_{k=0}^{118} \binom{118}{k} x^k \
(x + 1)^{119} = \sum_{k=0}^{119} \binom{119}{k} x^k \
(x + 1)^{120} = \sum_{k=0}^{120} \binom{120}{k} x^k \
\end{align*}

\subsection*{Derivative Table}
\begin{align*}
\frac{d}{dx} x^{1} = 1x^{0} \
\frac{d}{dx} x^{2} = 2x^{1} \
\frac{d}{dx} x^{3} = 3x^{2} \
\frac{d}{dx} x^{4} = 4x^{3} \
\frac{d}{dx} x^{5} = 5x^{4} \
\frac{d}{dx} x^{6} = 6x^{5} \
\frac{d}{dx} x^{7} = 7x^{6} \
\frac{d}{dx} x^{8} = 8x^{7} \
\frac{d}{dx} x^{9} = 9x^{8} \
\frac{d}{dx} x^{10} = 10x^{9} \
\frac{d}{dx} x^{11} = 11x^{10} \
\frac{d}{dx} x^{12} = 12x^{11} \
\frac{d}{dx} x^{13} = 13x^{12} \
\frac{d}{dx} x^{14} = 14x^{13} \
\frac{d}{dx} x^{15} = 15x^{14} \
\frac{d}{dx} x^{16} = 16x^{15} \
\frac{d}{dx} x^{17} = 17x^{16} \
\frac{d}{dx} x^{18} = 18x^{17} \
\frac{d}{dx} x^{19} = 19x^{18} \
\frac{d}{dx} x^{20} = 20x^{19} \
\frac{d}{dx} x^{21} = 21x^{20} \
\frac{d}{dx} x^{22} = 22x^{21} \
\frac{d}{dx} x^{23} = 23x^{22} \
\frac{d}{dx} x^{24} = 24x^{23} \
\frac{d}{dx} x^{25} = 25x^{24} \
\frac{d}{dx} x^{26} = 26x^{25} \
\frac{d}{dx} x^{27} = 27x^{26} \
\frac{d}{dx} x^{28} = 28x^{27} \
\frac{d}{dx} x^{29} = 29x^{28} \
\frac{d}{dx} x^{30} = 30x^{29} \
\frac{d}{dx} x^{31} = 31x^{30} \
\frac{d}{dx} x^{32} = 32x^{31} \
\frac{d}{dx} x^{33} = 33x^{32} \
\frac{d}{dx} x^{34} = 34x^{33} \
\frac{d}{dx} x^{35} = 35x^{34} \
\frac{d}{dx} x^{36} = 36x^{35} \
\frac{d}{dx} x^{37} = 37x^{36} \
\frac{d}{dx} x^{38} = 38x^{37} \
\frac{d}{dx} x^{39} = 39x^{38} \
\frac{d}{dx} x^{40} = 40x^{39} \
\frac{d}{dx} x^{41} = 41x^{40} \
\frac{d}{dx} x^{42} = 42x^{41} \
\frac{d}{dx} x^{43} = 43x^{42} \
\frac{d}{dx} x^{44} = 44x^{43} \
\frac{d}{dx} x^{45} = 45x^{44} \
\frac{d}{dx} x^{46} = 46x^{45} \
\frac{d}{dx} x^{47} = 47x^{46} \
\frac{d}{dx} x^{48} = 48x^{47} \
\frac{d}{dx} x^{49} = 49x^{48} \
\frac{d}{dx} x^{50} = 50x^{49} \
\frac{d}{dx} x^{51} = 51x^{50} \
\frac{d}{dx} x^{52} = 52x^{51} \
\frac{d}{dx} x^{53} = 53x^{52} \
\frac{d}{dx} x^{54} = 54x^{53} \
\frac{d}{dx} x^{55} = 55x^{54} \
\frac{d}{dx} x^{56} = 56x^{55} \
\frac{d}{dx} x^{57} = 57x^{56} \
\frac{d}{dx} x^{58} = 58x^{57} \
\frac{d}{dx} x^{59} = 59x^{58} \
\frac{d}{dx} x^{60} = 60x^{59} \
\frac{d}{dx} x^{61} = 61x^{60} \
\frac{d}{dx} x^{62} = 62x^{61} \
\frac{d}{dx} x^{63} = 63x^{62} \
\frac{d}{dx} x^{64} = 64x^{63} \
\frac{d}{dx} x^{65} = 65x^{64} \
\frac{d}{dx} x^{66} = 66x^{65} \
\frac{d}{dx} x^{67} = 67x^{66} \
\frac{d}{dx} x^{68} = 68x^{67} \
\frac{d}{dx} x^{69} = 69x^{68} \
\frac{d}{dx} x^{70} = 70x^{69} \
\frac{d}{dx} x^{71} = 71x^{70} \
\frac{d}{dx} x^{72} = 72x^{71} \
\frac{d}{dx} x^{73} = 73x^{72} \
\frac{d}{dx} x^{74} = 74x^{73} \
\frac{d}{dx} x^{75} = 75x^{74} \
\frac{d}{dx} x^{76} = 76x^{75} \
\frac{d}{dx} x^{77} = 77x^{76} \
\frac{d}{dx} x^{78} = 78x^{77} \
\frac{d}{dx} x^{79} = 79x^{78} \
\frac{d}{dx} x^{80} = 80x^{79} \
\frac{d}{dx} x^{81} = 81x^{80} \
\frac{d}{dx} x^{82} = 82x^{81} \
\frac{d}{dx} x^{83} = 83x^{82} \
\frac{d}{dx} x^{84} = 84x^{83} \
\frac{d}{dx} x^{85} = 85x^{84} \
\frac{d}{dx} x^{86} = 86x^{85} \
\frac{d}{dx} x^{87} = 87x^{86} \
\frac{d}{dx} x^{88} = 88x^{87} \
\frac{d}{dx} x^{89} = 89x^{88} \
\frac{d}{dx} x^{90} = 90x^{89} \
\frac{d}{dx} x^{91} = 91x^{90} \
\frac{d}{dx} x^{92} = 92x^{91} \
\frac{d}{dx} x^{93} = 93x^{92} \
\frac{d}{dx} x^{94} = 94x^{93} \
\frac{d}{dx} x^{95} = 95x^{94} \
\frac{d}{dx} x^{96} = 96x^{95} \
\frac{d}{dx} x^{97} = 97x^{96} \
\frac{d}{dx} x^{98} = 98x^{97} \
\frac{d}{dx} x^{99} = 99x^{98} \
\frac{d}{dx} x^{100} = 100x^{99} \
\frac{d}{dx} x^{101} = 101x^{100} \
\frac{d}{dx} x^{102} = 102x^{101} \
\frac{d}{dx} x^{103} = 103x^{102} \
\frac{d}{dx} x^{104} = 104x^{103} \
\frac{d}{dx} x^{105} = 105x^{104} \
\frac{d}{dx} x^{106} = 106x^{105} \
\frac{d}{dx} x^{107} = 107x^{106} \
\frac{d}{dx} x^{108} = 108x^{107} \
\frac{d}{dx} x^{109} = 109x^{108} \
\frac{d}{dx} x^{110} = 110x^{109} \
\frac{d}{dx} x^{111} = 111x^{110} \
\frac{d}{dx} x^{112} = 112x^{111} \
\frac{d}{dx} x^{113} = 113x^{112} \
\frac{d}{dx} x^{114} = 114x^{113} \
\frac{d}{dx} x^{115} = 115x^{114} \
\frac{d}{dx} x^{116} = 116x^{115} \
\frac{d}{dx} x^{117} = 117x^{116} \
\frac{d}{dx} x^{118} = 118x^{117} \
\frac{d}{dx} x^{119} = 119x^{118} \
\frac{d}{dx} x^{120} = 120x^{119} \
\end{align*}
