% Auto-generated equations for trigonometry.
% This file is maintained by EquationGenerator.

\section*{Trigonometry}
\begin{align*}
\text{Example 1:}\quad \sin(1\theta)^2 + \cos(1\theta)^2 = 1 \
\text{Example 2:}\quad \sin(2\theta)^2 + \cos(2\theta)^2 = 1 \
\text{Example 3:}\quad \sin(3\theta)^2 + \cos(3\theta)^2 = 1 \
\text{Example 4:}\quad \sin(4\theta)^2 + \cos(4\theta)^2 = 1 \
\text{Example 5:}\quad \sin(5\theta)^2 + \cos(5\theta)^2 = 1 \
\text{Example 6:}\quad \sin(6\theta)^2 + \cos(6\theta)^2 = 1 \
\text{Example 7:}\quad \sin(7\theta)^2 + \cos(7\theta)^2 = 1 \
\text{Example 8:}\quad \sin(8\theta)^2 + \cos(8\theta)^2 = 1 \
\text{Example 9:}\quad \sin(9\theta)^2 + \cos(9\theta)^2 = 1 \
\text{Example 10:}\quad \sin(10\theta)^2 + \cos(10\theta)^2 = 1 \
\text{Example 11:}\quad \sin(11\theta)^2 + \cos(11\theta)^2 = 1 \
\text{Example 12:}\quad \sin(12\theta)^2 + \cos(12\theta)^2 = 1 \
\text{Example 13:}\quad \sin(13\theta)^2 + \cos(13\theta)^2 = 1 \
\text{Example 14:}\quad \sin(14\theta)^2 + \cos(14\theta)^2 = 1 \
\text{Example 15:}\quad \sin(15\theta)^2 + \cos(15\theta)^2 = 1 \
\text{Example 16:}\quad \sin(16\theta)^2 + \cos(16\theta)^2 = 1 \
\text{Example 17:}\quad \sin(17\theta)^2 + \cos(17\theta)^2 = 1 \
\text{Example 18:}\quad \sin(18\theta)^2 + \cos(18\theta)^2 = 1 \
\text{Example 19:}\quad \sin(19\theta)^2 + \cos(19\theta)^2 = 1 \
\text{Example 20:}\quad \sin(20\theta)^2 + \cos(20\theta)^2 = 1 \
\text{Example 21:}\quad \sin(21\theta)^2 + \cos(21\theta)^2 = 1 \
\text{Example 22:}\quad \sin(22\theta)^2 + \cos(22\theta)^2 = 1 \
\text{Example 23:}\quad \sin(23\theta)^2 + \cos(23\theta)^2 = 1 \
\text{Example 24:}\quad \sin(24\theta)^2 + \cos(24\theta)^2 = 1 \
\text{Example 25:}\quad \sin(25\theta)^2 + \cos(25\theta)^2 = 1 \
\text{Example 26:}\quad \sin(26\theta)^2 + \cos(26\theta)^2 = 1 \
\text{Example 27:}\quad \sin(27\theta)^2 + \cos(27\theta)^2 = 1 \
\text{Example 28:}\quad \sin(28\theta)^2 + \cos(28\theta)^2 = 1 \
\text{Example 29:}\quad \sin(29\theta)^2 + \cos(29\theta)^2 = 1 \
\text{Example 30:}\quad \sin(30\theta)^2 + \cos(30\theta)^2 = 1 \
\text{Example 31:}\quad \sin(31\theta)^2 + \cos(31\theta)^2 = 1 \
\text{Example 32:}\quad \sin(32\theta)^2 + \cos(32\theta)^2 = 1 \
\text{Example 33:}\quad \sin(33\theta)^2 + \cos(33\theta)^2 = 1 \
\text{Example 34:}\quad \sin(34\theta)^2 + \cos(34\theta)^2 = 1 \
\text{Example 35:}\quad \sin(35\theta)^2 + \cos(35\theta)^2 = 1 \
\text{Example 36:}\quad \sin(36\theta)^2 + \cos(36\theta)^2 = 1 \
\text{Example 37:}\quad \sin(37\theta)^2 + \cos(37\theta)^2 = 1 \
\text{Example 38:}\quad \sin(38\theta)^2 + \cos(38\theta)^2 = 1 \
\text{Example 39:}\quad \sin(39\theta)^2 + \cos(39\theta)^2 = 1 \
\text{Example 40:}\quad \sin(40\theta)^2 + \cos(40\theta)^2 = 1 \
\text{Example 41:}\quad \sin(41\theta)^2 + \cos(41\theta)^2 = 1 \
\text{Example 42:}\quad \sin(42\theta)^2 + \cos(42\theta)^2 = 1 \
\text{Example 43:}\quad \sin(43\theta)^2 + \cos(43\theta)^2 = 1 \
\text{Example 44:}\quad \sin(44\theta)^2 + \cos(44\theta)^2 = 1 \
\text{Example 45:}\quad \sin(45\theta)^2 + \cos(45\theta)^2 = 1 \
\text{Example 46:}\quad \sin(46\theta)^2 + \cos(46\theta)^2 = 1 \
\text{Example 47:}\quad \sin(47\theta)^2 + \cos(47\theta)^2 = 1 \
\text{Example 48:}\quad \sin(48\theta)^2 + \cos(48\theta)^2 = 1 \
\text{Example 49:}\quad \sin(49\theta)^2 + \cos(49\theta)^2 = 1 \
\text{Example 50:}\quad \sin(50\theta)^2 + \cos(50\theta)^2 = 1 \
\text{Example 51:}\quad \sin(51\theta)^2 + \cos(51\theta)^2 = 1 \
\text{Example 52:}\quad \sin(52\theta)^2 + \cos(52\theta)^2 = 1 \
\text{Example 53:}\quad \sin(53\theta)^2 + \cos(53\theta)^2 = 1 \
\text{Example 54:}\quad \sin(54\theta)^2 + \cos(54\theta)^2 = 1 \
\text{Example 55:}\quad \sin(55\theta)^2 + \cos(55\theta)^2 = 1 \
\text{Example 56:}\quad \sin(56\theta)^2 + \cos(56\theta)^2 = 1 \
\text{Example 57:}\quad \sin(57\theta)^2 + \cos(57\theta)^2 = 1 \
\text{Example 58:}\quad \sin(58\theta)^2 + \cos(58\theta)^2 = 1 \
\text{Example 59:}\quad \sin(59\theta)^2 + \cos(59\theta)^2 = 1 \
\text{Example 60:}\quad \sin(60\theta)^2 + \cos(60\theta)^2 = 1 \
\text{Example 61:}\quad \sin(61\theta)^2 + \cos(61\theta)^2 = 1 \
\text{Example 62:}\quad \sin(62\theta)^2 + \cos(62\theta)^2 = 1 \
\text{Example 63:}\quad \sin(63\theta)^2 + \cos(63\theta)^2 = 1 \
\text{Example 64:}\quad \sin(64\theta)^2 + \cos(64\theta)^2 = 1 \
\text{Example 65:}\quad \sin(65\theta)^2 + \cos(65\theta)^2 = 1 \
\text{Example 66:}\quad \sin(66\theta)^2 + \cos(66\theta)^2 = 1 \
\text{Example 67:}\quad \sin(67\theta)^2 + \cos(67\theta)^2 = 1 \
\text{Example 68:}\quad \sin(68\theta)^2 + \cos(68\theta)^2 = 1 \
\text{Example 69:}\quad \sin(69\theta)^2 + \cos(69\theta)^2 = 1 \
\text{Example 70:}\quad \sin(70\theta)^2 + \cos(70\theta)^2 = 1 \
\text{Example 71:}\quad \sin(71\theta)^2 + \cos(71\theta)^2 = 1 \
\text{Example 72:}\quad \sin(72\theta)^2 + \cos(72\theta)^2 = 1 \
\text{Example 73:}\quad \sin(73\theta)^2 + \cos(73\theta)^2 = 1 \
\text{Example 74:}\quad \sin(74\theta)^2 + \cos(74\theta)^2 = 1 \
\text{Example 75:}\quad \sin(75\theta)^2 + \cos(75\theta)^2 = 1 \
\text{Example 76:}\quad \sin(76\theta)^2 + \cos(76\theta)^2 = 1 \
\text{Example 77:}\quad \sin(77\theta)^2 + \cos(77\theta)^2 = 1 \
\text{Example 78:}\quad \sin(78\theta)^2 + \cos(78\theta)^2 = 1 \
\text{Example 79:}\quad \sin(79\theta)^2 + \cos(79\theta)^2 = 1 \
\text{Example 80:}\quad \sin(80\theta)^2 + \cos(80\theta)^2 = 1 \
\text{Example 81:}\quad \sin(81\theta)^2 + \cos(81\theta)^2 = 1 \
\text{Example 82:}\quad \sin(82\theta)^2 + \cos(82\theta)^2 = 1 \
\text{Example 83:}\quad \sin(83\theta)^2 + \cos(83\theta)^2 = 1 \
\text{Example 84:}\quad \sin(84\theta)^2 + \cos(84\theta)^2 = 1 \
\text{Example 85:}\quad \sin(85\theta)^2 + \cos(85\theta)^2 = 1 \
\text{Example 86:}\quad \sin(86\theta)^2 + \cos(86\theta)^2 = 1 \
\text{Example 87:}\quad \sin(87\theta)^2 + \cos(87\theta)^2 = 1 \
\text{Example 88:}\quad \sin(88\theta)^2 + \cos(88\theta)^2 = 1 \
\text{Example 89:}\quad \sin(89\theta)^2 + \cos(89\theta)^2 = 1 \
\text{Example 90:}\quad \sin(90\theta)^2 + \cos(90\theta)^2 = 1 \
\text{Example 91:}\quad \sin(91\theta)^2 + \cos(91\theta)^2 = 1 \
\text{Example 92:}\quad \sin(92\theta)^2 + \cos(92\theta)^2 = 1 \
\text{Example 93:}\quad \sin(93\theta)^2 + \cos(93\theta)^2 = 1 \
\text{Example 94:}\quad \sin(94\theta)^2 + \cos(94\theta)^2 = 1 \
\text{Example 95:}\quad \sin(95\theta)^2 + \cos(95\theta)^2 = 1 \
\text{Example 96:}\quad \sin(96\theta)^2 + \cos(96\theta)^2 = 1 \
\text{Example 97:}\quad \sin(97\theta)^2 + \cos(97\theta)^2 = 1 \
\text{Example 98:}\quad \sin(98\theta)^2 + \cos(98\theta)^2 = 1 \
\text{Example 99:}\quad \sin(99\theta)^2 + \cos(99\theta)^2 = 1 \
\text{Example 100:}\quad \sin(100\theta)^2 + \cos(100\theta)^2 = 1 \
\text{Example 101:}\quad \sin(101\theta)^2 + \cos(101\theta)^2 = 1 \
\text{Example 102:}\quad \sin(102\theta)^2 + \cos(102\theta)^2 = 1 \
\text{Example 103:}\quad \sin(103\theta)^2 + \cos(103\theta)^2 = 1 \
\text{Example 104:}\quad \sin(104\theta)^2 + \cos(104\theta)^2 = 1 \
\text{Example 105:}\quad \sin(105\theta)^2 + \cos(105\theta)^2 = 1 \
\text{Example 106:}\quad \sin(106\theta)^2 + \cos(106\theta)^2 = 1 \
\text{Example 107:}\quad \sin(107\theta)^2 + \cos(107\theta)^2 = 1 \
\text{Example 108:}\quad \sin(108\theta)^2 + \cos(108\theta)^2 = 1 \
\text{Example 109:}\quad \sin(109\theta)^2 + \cos(109\theta)^2 = 1 \
\text{Example 110:}\quad \sin(110\theta)^2 + \cos(110\theta)^2 = 1 \
\text{Example 111:}\quad \sin(111\theta)^2 + \cos(111\theta)^2 = 1 \
\text{Example 112:}\quad \sin(112\theta)^2 + \cos(112\theta)^2 = 1 \
\text{Example 113:}\quad \sin(113\theta)^2 + \cos(113\theta)^2 = 1 \
\text{Example 114:}\quad \sin(114\theta)^2 + \cos(114\theta)^2 = 1 \
\text{Example 115:}\quad \sin(115\theta)^2 + \cos(115\theta)^2 = 1 \
\text{Example 116:}\quad \sin(116\theta)^2 + \cos(116\theta)^2 = 1 \
\text{Example 117:}\quad \sin(117\theta)^2 + \cos(117\theta)^2 = 1 \
\text{Example 118:}\quad \sin(118\theta)^2 + \cos(118\theta)^2 = 1 \
\text{Example 119:}\quad \sin(119\theta)^2 + \cos(119\theta)^2 = 1 \
\text{Example 120:}\quad \sin(120\theta)^2 + \cos(120\theta)^2 = 1 \
\text{Example 121:}\quad \sin(121\theta)^2 + \cos(121\theta)^2 = 1 \
\text{Example 122:}\quad \sin(122\theta)^2 + \cos(122\theta)^2 = 1 \
\text{Example 123:}\quad \sin(123\theta)^2 + \cos(123\theta)^2 = 1 \
\text{Example 124:}\quad \sin(124\theta)^2 + \cos(124\theta)^2 = 1 \
\text{Example 125:}\quad \sin(125\theta)^2 + \cos(125\theta)^2 = 1 \
\text{Example 126:}\quad \sin(126\theta)^2 + \cos(126\theta)^2 = 1 \
\text{Example 127:}\quad \sin(127\theta)^2 + \cos(127\theta)^2 = 1 \
\text{Example 128:}\quad \sin(128\theta)^2 + \cos(128\theta)^2 = 1 \
\text{Example 129:}\quad \sin(129\theta)^2 + \cos(129\theta)^2 = 1 \
\text{Example 130:}\quad \sin(130\theta)^2 + \cos(130\theta)^2 = 1 \
\text{Example 131:}\quad \sin(131\theta)^2 + \cos(131\theta)^2 = 1 \
\text{Example 132:}\quad \sin(132\theta)^2 + \cos(132\theta)^2 = 1 \
\text{Example 133:}\quad \sin(133\theta)^2 + \cos(133\theta)^2 = 1 \
\text{Example 134:}\quad \sin(134\theta)^2 + \cos(134\theta)^2 = 1 \
\text{Example 135:}\quad \sin(135\theta)^2 + \cos(135\theta)^2 = 1 \
\text{Example 136:}\quad \sin(136\theta)^2 + \cos(136\theta)^2 = 1 \
\text{Example 137:}\quad \sin(137\theta)^2 + \cos(137\theta)^2 = 1 \
\text{Example 138:}\quad \sin(138\theta)^2 + \cos(138\theta)^2 = 1 \
\text{Example 139:}\quad \sin(139\theta)^2 + \cos(139\theta)^2 = 1 \
\text{Example 140:}\quad \sin(140\theta)^2 + \cos(140\theta)^2 = 1 \
\text{Example 141:}\quad \sin(141\theta)^2 + \cos(141\theta)^2 = 1 \
\text{Example 142:}\quad \sin(142\theta)^2 + \cos(142\theta)^2 = 1 \
\text{Example 143:}\quad \sin(143\theta)^2 + \cos(143\theta)^2 = 1 \
\text{Example 144:}\quad \sin(144\theta)^2 + \cos(144\theta)^2 = 1 \
\text{Example 145:}\quad \sin(145\theta)^2 + \cos(145\theta)^2 = 1 \
\text{Example 146:}\quad \sin(146\theta)^2 + \cos(146\theta)^2 = 1 \
\text{Example 147:}\quad \sin(147\theta)^2 + \cos(147\theta)^2 = 1 \
\text{Example 148:}\quad \sin(148\theta)^2 + \cos(148\theta)^2 = 1 \
\text{Example 149:}\quad \sin(149\theta)^2 + \cos(149\theta)^2 = 1 \
\text{Example 150:}\quad \sin(150\theta)^2 + \cos(150\theta)^2 = 1 \
\text{Example 151:}\quad \sin(151\theta)^2 + \cos(151\theta)^2 = 1 \
\text{Example 152:}\quad \sin(152\theta)^2 + \cos(152\theta)^2 = 1 \
\text{Example 153:}\quad \sin(153\theta)^2 + \cos(153\theta)^2 = 1 \
\text{Example 154:}\quad \sin(154\theta)^2 + \cos(154\theta)^2 = 1 \
\text{Example 155:}\quad \sin(155\theta)^2 + \cos(155\theta)^2 = 1 \
\text{Example 156:}\quad \sin(156\theta)^2 + \cos(156\theta)^2 = 1 \
\text{Example 157:}\quad \sin(157\theta)^2 + \cos(157\theta)^2 = 1 \
\text{Example 158:}\quad \sin(158\theta)^2 + \cos(158\theta)^2 = 1 \
\text{Example 159:}\quad \sin(159\theta)^2 + \cos(159\theta)^2 = 1 \
\text{Example 160:}\quad \sin(160\theta)^2 + \cos(160\theta)^2 = 1 \
\text{Example 161:}\quad \sin(161\theta)^2 + \cos(161\theta)^2 = 1 \
\text{Example 162:}\quad \sin(162\theta)^2 + \cos(162\theta)^2 = 1 \
\text{Example 163:}\quad \sin(163\theta)^2 + \cos(163\theta)^2 = 1 \
\text{Example 164:}\quad \sin(164\theta)^2 + \cos(164\theta)^2 = 1 \
\text{Example 165:}\quad \sin(165\theta)^2 + \cos(165\theta)^2 = 1 \
\text{Example 166:}\quad \sin(166\theta)^2 + \cos(166\theta)^2 = 1 \
\text{Example 167:}\quad \sin(167\theta)^2 + \cos(167\theta)^2 = 1 \
\text{Example 168:}\quad \sin(168\theta)^2 + \cos(168\theta)^2 = 1 \
\text{Example 169:}\quad \sin(169\theta)^2 + \cos(169\theta)^2 = 1 \
\text{Example 170:}\quad \sin(170\theta)^2 + \cos(170\theta)^2 = 1 \
\text{Example 171:}\quad \sin(171\theta)^2 + \cos(171\theta)^2 = 1 \
\text{Example 172:}\quad \sin(172\theta)^2 + \cos(172\theta)^2 = 1 \
\text{Example 173:}\quad \sin(173\theta)^2 + \cos(173\theta)^2 = 1 \
\text{Example 174:}\quad \sin(174\theta)^2 + \cos(174\theta)^2 = 1 \
\text{Example 175:}\quad \sin(175\theta)^2 + \cos(175\theta)^2 = 1 \
\text{Example 176:}\quad \sin(176\theta)^2 + \cos(176\theta)^2 = 1 \
\text{Example 177:}\quad \sin(177\theta)^2 + \cos(177\theta)^2 = 1 \
\text{Example 178:}\quad \sin(178\theta)^2 + \cos(178\theta)^2 = 1 \
\text{Example 179:}\quad \sin(179\theta)^2 + \cos(179\theta)^2 = 1 \
\text{Example 180:}\quad \sin(180\theta)^2 + \cos(180\theta)^2 = 1 \
\end{align*}
